Tasks - meeting 2020 06 10 (#12)
* Removing all "Compute generate_dot [...]" commands

* Updating contextual rule for specification record

* Removing the trace examples that have been proved manually

* Standardizing specification names

* Defining traces model (relation)

* Attempting to prove compute_ltsR_correctness theorem (ProcRef constructor subgoal)

Coq/CSP/lts.v
@@ -41,10 +41,10 @@ Inductive ltsR' :
   set proc_body -> (* the states still to be visited *)
   set proc_body -> (* the visited states *)
   Prop :=
-  | lts_empty_rule (C : specification) (visited : set proc_body) :
-      ltsR' C nil nil visited
+  | lts_empty_rule (S : specification) (visited : set proc_body) :
+      ltsR' S nil nil visited
   | lts_inductive_rule
-        (C : specification)
+        (S : specification)
         (T : set transition)
         (P : proc_body)
         (tl visited : set proc_body) :
@@ -55,13 +55,13 @@ Inductive ltsR' :
                         (set_union proc_body_eq_dec tl (target_proc_bodies T'))
                         visited' in
       (forall (a : event_tau_tick) (P' : proc_body),
-         (C # P // a ==> P') <-> In (P,a,P') T') ->
-      ltsR' C T'' to_visit visited' ->
-      ltsR' C T (P :: tl) visited.
+         (S # P // a ==> P') <-> In (P,a,P') T') ->
+      ltsR' S T'' to_visit visited' ->
+      ltsR' S T (P :: tl) visited.
 
-Definition ltsR (C : specification) (T : set transition) (name : string) : Prop :=
-  match get_proc_body C name with
-  | Some body => NoDup T /\ ltsR' C T [body] nil
+Definition ltsR (S : specification) (T : set transition) (name : string) : Prop :=
+  match get_proc_body S name with
+  | Some body => NoDup T /\ ltsR' S T [body] nil
   | None => False
   end.
 
@@ -243,10 +243,10 @@ Theorem compute_ltsR_step_more:
 Proof. Admitted.
 
 Theorem compute_ltsR_correctness:
-  forall (spec : specification) (proc_id : string) (n : nat) (trans_set : set transition),
-  compute_ltsR spec proc_id n = Some trans_set -> ltsR spec trans_set proc_id.
+  forall (S : specification) (proc_id : string) (n : nat) (trans_set : set transition),
+  compute_ltsR S proc_id n = Some trans_set -> ltsR S trans_set proc_id.
 Proof.
-  intros. destruct (get_proc_body spec proc_id) eqn:H1.
+  intros. destruct (get_proc_body S proc_id) eqn:H1.
   - destruct p.
     * (* SKIP *)
       unfold compute_ltsR in H; rewrite -> H1 in H. destruct n.
@@ -348,11 +348,44 @@ Proof.
             simpl. apply lts_empty_rule. 
           }
         }
-    * (* ProcRef name *) admit.
+    * (* ProcRef name *)
+      unfold ltsR. rewrite -> H1. split.
+      + unfold compute_ltsR in H. rewrite -> H1 in H.
+        induction n.
+        { inversion H. }
+        {
+          inversion H. destruct (get_proc_body S name) eqn:H3.
+          {
+            inversion H2. destruct (compute_ltsR' S [p] [ProcRef name] n) eqn:H5.
+            {
+              inversion H4. induction s.
+              { simpl. solve_nodup. }
+              { unfold set_union. unfold set_add. admit. }
+            }
+            { inversion H4. }
+          }
+          { inversion H2. admit. }
+        }
+      + apply lts_inductive_rule.
+        {
+          split.
+          {
+            intros. inversion H0; subst. unfold compute_ltsR in H; rewrite -> H1 in H.
+            destruct n.
+            { inversion H. }
+            { 
+              inversion H. destruct (get_proc_body S name).
+              { inversion H5. admit. }
+              admit.
+            }
+          }
+          admit.
+        }
+        admit.
     * (* e --> P *)
       unfold compute_ltsR in H; rewrite -> H1 in H. induction n.
       + inversion H.
-      + inversion H. destruct (compute_ltsR' spec [p] [event --> p] n) eqn:H3.
+      + inversion H. destruct (compute_ltsR' S [p] [event --> p] n) eqn:H3.
         {
           induction s.
           {
@@ -434,20 +467,16 @@ Proof.
     ]
   ).
 Defined.
-Compute generate_dot (compute_ltsR S_FORECOURT "FORECOURT" 100).
 
 Definition TOY' : specification.
 Proof.
   solve_spec_ctx_rules (Build_Spec [Channel {{"a", "b"}}] ["P" ::= "b" --> SKIP [] "a" --> STOP \ {{"a"}}]).
 Defined.
-Compute generate_dot( compute_ltsR TOY' "P" 10).
 
 Definition CH := Channel {{"a", "b"}}.
 Definition P := "P" ::= "a" --> STOP [] "b" --> "b" --> STOP.
 Definition S : specification.
 Proof. solve_spec_ctx_rules (Build_Spec [CH] [P]). Defined.
-
-Compute generate_dot (compute_ltsR S "P" 100).
 
 Definition CH_TEAM := Channel {{"lift_piano", "lift_table"}}.
 Definition PETE := "PETE" ::= "lift_piano" --> ProcRef "PETE"
@@ -461,12 +490,8 @@ Definition TEAM := "TEAM" ::= ProcRef "PETE" [| {{"lift_piano", "lift_table"}} |
 Definition S_TEAM : specification.
 Proof. solve_spec_ctx_rules (Build_Spec [CH_TEAM] [PETE ; DAVE ; TEAM]). Defined.
 
-Compute generate_dot (compute_ltsR S_TEAM "TEAM" 100).
-
 Definition TOY_PROBLEM : specification.
 Proof. solve_spec_ctx_rules (Build_Spec [Channel {{"a", "b"}}] ["P" ::= "a" --> "b" --> STOP]). Defined.
-
-Compute generate_dot (compute_ltsR TOY_PROBLEM "P" 100).
 
 Example lts1 :
   ltsR
@@ -517,8 +542,6 @@ Proof.
     ["P" ::= ("a" --> "b" --> STOP) [] ("c" --> STOP)]
   ).
 Defined.
-
-Compute generate_dot (compute_ltsR TOY_PROBLEM' "P" 100).
 
 Example lts2 :
   ltsR
@@ -586,8 +609,6 @@ Definition P' := "P" ::= ProcRef "P".
 Definition UNDERDEFINED_RECURSION : specification.
 Proof. solve_spec_ctx_rules (Build_Spec [Channel {{}}] [P']). Defined.
 
-Compute generate_dot (compute_ltsR UNDERDEFINED_RECURSION "P" 100).
-
 Example lts3 : ltsR UNDERDEFINED_RECURSION [(ProcRef "P", Tau, ProcRef "P")] "P".
 Proof.
   unfold ltsR. split.
@@ -613,8 +634,6 @@ Definition S_LIGHT : specification.
 Proof.
   solve_spec_ctx_rules (Build_Spec [Channel {{"on", "off"}}] ["LIGHT" ::= "on" --> "off" --> ProcRef "LIGHT"]).
 Defined.
-
-Compute generate_dot (compute_ltsR S_LIGHT "LIGHT" 100).
 
 Example lts4 :
   ltsR
@@ -679,8 +698,6 @@ Definition PARKING_PERMIT_MCH : specification.
 Proof.
   solve_spec_ctx_rules (Build_Spec [Channel {{"cash", "ticket", "change"}}] [TICKET ; CHANGE ; MACHINE]).
 Defined.
-
-Compute generate_dot (compute_ltsR PARKING_PERMIT_MCH "MACHINE" 100).
 
 (*
 Example lts5 :
